{
  "@context": {
    "dct": "http://purl.org/dc/terms/",
    "owl": "http://www.w3.org/2002/07/owl#",
    "rdf": "http://www.w3.org/1999/02/22-rdf-syntax-ns#",
    "rdfa": "http://www.w3.org/ns/rdfa#",
    "rdfs": "http://www.w3.org/2000/01/rdf-schema#",
    "schema": "http://schema.org/",
    "xsd": "http://www.w3.org/2001/XMLSchema#",
    "cvisb": "https://data.cvisb.org/jsonschema/"
  },
  "version": 0.1,
  "@id": "https://data.cvisb.org/jsonschema/v0.1",
  "@graph": [
    {
      "@id": "cvisb:Patient",
      "@type": "rdfs:Class",
      "rdfs:comment": "A schema describing a Patient/Person in the Center for Viral Systems Biology experiments",
      "rdfs:label": "Patient",
      "rdfs:subClassOf": {
        "@id": "health:Patient"
      },
      "schema:isPartOf": {
        "@id": "https://data.cvisb.org/schema"
      },
      "root_entity": true
    },
    {
      "@id": "cvisb:patientID",
      "@type": "rdf:Property",
      "rdfs:comment": "Unique, public study ID for patient",
      "rdfs:label": "patientID",
      "schema:domainIncludes": [
        {
          "@id": "cvisb:Patient"
        }
      ],
      "schema:rangeIncludes": [
        {
          "@id": "schema:Text"
        }
      ],
      "schema:sameAs": {
        "@id": "schema:identifier"
      },
      "owl:cardinality": "one",
      "marginality": "required",
      "authenticated": false
    },
    {
      "@id": "cvisb:species",
      "@type": "rdf:Property",
      "rdfs:comment": "Species of patient (Homo sapiens, Hylomyscus pamfi, Mastomys erythroleucus, Mastomys natalensis, rodent, etc)",
      "rdfs:label": "species",
      "schema:domainIncludes": [
        {
          "@id": "cvisb:Patient"
        }
      ],
      "schema:rangeIncludes": [
        {
          "@id": "xsd:string"
        },
        {
          "@id": "schema:Text"
        }
      ],
      "owl:cardinality": "one",
      "marginality": "recommended",
      "schema:Enumeration": [
        "Homo sapiens",
        "Hylomyscus pamfi",
        "Mastomys erythroleucus",
        "Mastomys natalensis",
        "rodent",
        null
      ],
      "authenticated": false
    },
    {
      "@id": "cvisb:alternateIdentifier",
      "@type": "rdf:Property",
      "rdfs:comment": "Alternative ID(s) used for patient (including G-number, S-number, or C-numbers, available to consortia members only)",
      "rdfs:label": "alternateIdentifier",
      "schema:domainIncludes": [
        {
          "@id": "cvisb:Patient"
        }
      ],
      "schema:rangeIncludes": [
        {
          "@id": "schema:Text"
        }
      ],
      "owl:cardinality": "many",
      "marginality": "optional",
      "authenticated": true
    },
    {
      "@id": "cvisb:gID",
      "@type": "rdf:Property",
      "rdfs:comment": "Internal G-number used to refer to the patients when they're in the acute treatment phase at KGH. For most samples, should be a single gID; however, some patients have two.",
      "rdfs:label": "gID",
      "schema:domainIncludes": [
        {
          "@id": "cvisb:Patient"
        }
      ],
      "schema:rangeIncludes": [
        {
          "@id": "schema:Text"
        }
      ],
      "owl:cardinality": "many",
      "marginality": "optional",
      "authenticated": true
    },
    {
      "@id": "cvisb:hasPatientData",
      "@type": "rdf:Property",
      "rdfs:comment": "Whether CViSB has data, metadata, and/or samples from the acute phase of infection of the patient.",
      "rdfs:label": "hasPatientData",
      "schema:domainIncludes": [
        {
          "@id": "cvisb:Patient"
        }
      ],
      "schema:rangeIncludes": [
        {
          "@id": "schema:Boolean"
        }
      ],
      "owl:cardinality": "one",
      "marginality": "optional",
      "authenticated": true
    },
    {
      "@id": "cvisb:sID",
      "@type": "rdf:Property",
      "rdfs:comment": "Internal survivor ID used to refer to the patients during follow-up visits. Can include either survivors (S-numbers) or contacts (C-numbers)",
      "rdfs:label": "sID",
      "schema:domainIncludes": [
        {
          "@id": "cvisb:Patient"
        }
      ],
      "schema:rangeIncludes": [
        {
          "@id": "schema:Text"
        }
      ],
      "owl:cardinality": "one",
      "marginality": "optional",
      "authenticated": true
    },
    {
      "@id": "cvisb:hasSurvivorData",
      "@type": "rdf:Property",
      "rdfs:comment": "Whether CViSB has data, metadata, and/or samples from follow-up visits after the patient has survived the acute infection phase.",
      "rdfs:label": "hasSurvivorData",
      "schema:domainIncludes": [
        {
          "@id": "cvisb:Patient"
        }
      ],
      "schema:rangeIncludes": [
        {
          "@id": "schema:Boolean"
        }
      ],
      "owl:cardinality": "one",
      "marginality": "optional",
      "authenticated": true
    },
    {
      "@id": "cvisb:contactGroupIdentifier",
      "@type": "rdf:Property",
      "rdfs:comment": "ID group for patient and associated contacts",
      "rdfs:label": "contactGroupIdentifier",
      "schema:domainIncludes": [
        {
          "@id": "cvisb:Patient"
        }
      ],
      "schema:rangeIncludes": [
        {
          "@id": "schema:Text"
        }
      ],
      "owl:cardinality": "one",
      "marginality": "recommended",
      "authenticated": true
    },
    {
      "@id": "cvisb:dateModified",
      "@type": "rdf:Property",
      "rdfs:comment": "Date on which the Patient metadata was most recently modified",
      "rdfs:label": "dateModified",
      "schema:domainIncludes": [
        {
          "@id": "cvisb:Patient"
        }
      ],
      "schema:rangeIncludes": [
        {
          "@id": "schema:Date"
        }
      ],
      "schema:sameAs": {
        "@id": "schema:dateModified"
      },
      "owl:cardinality": "one",
      "marginality": "required",
      "authenticated": false
    },
    {
      "@id": "cvisb:updatedBy",
      "@type": "rdf:Property",
      "rdfs:comment": "Person who updated the patient data",
      "rdfs:label": "updatedBy",
      "schema:domainIncludes": [
        {
          "@id": "cvisb:Patient"
        }
      ],
      "schema:rangeIncludes": [
        {
          "@id": "xsd:string"
        },
        {
          "@id": "schema:Text"
        }
      ],
      "owl:cardinality": "one",
      "marginality": "recommended",
      "authenticated": true
    },
    {
      "@id": "cvisb:dataStatus",
      "@type": "rdf:Property",
      "rdfs:comment": "description of whether the data is considered preliminary (subject to review) or finalized. Note that \"final\" data can still be modified.",
      "rdfs:label": "dataStatus",
      "schema:domainIncludes": [
        {
          "@id": "cvisb:Patient"
        }
      ],
      "schema:rangeIncludes": [
        {
          "@id": "schema:Text"
        }
      ],
      "owl:cardinality": "one",
      "marginality": "recommended",
      "authenticated": false,
      "schema:Enumeration": [
        "preliminary",
        "final"
      ]
    },
    {
      "@id": "cvisb:sourceFiles",
      "@type": "rdf:Property",
      "rdfs:comment": "Internal tracking of who / which file(s) supplied the patient metadata",
      "rdfs:label": "sourceFiles",
      "schema:domainIncludes": [
        {
          "@id": "cvisb:Patient"
        }
      ],
      "schema:rangeIncludes": [
        {
          "@id": "xsd:string"
        },
        {
          "@id": "schema:Text"
        }
      ],
      "owl:cardinality": "many",
      "marginality": "recommended",
      "authenticated": true
    },
    {
      "@id": "cvisb:version",
      "@type": "rdf:Property",
      "rdfs:comment": "Version number of patient data",
      "rdfs:label": "version",
      "schema:domainIncludes": [
        {
          "@id": "cvisb:Patient"
        }
      ],
      "schema:rangeIncludes": [
        {
          "@id": "schema:Number"
        }
      ],
      "schema:sameAs": {
        "@id": "schema:version"
      },
      "owl:cardinality": "one",
      "marginality": "recommended",
      "authenticated": false
    },
    {
      "@id": "cvisb:cohort",
      "@type": "rdf:Property",
      "rdfs:comment": "Cohort for virus exposure: Ebola, Lassa, COVID-19, or control.  Note that this is not a diagnosis, but rather what the patient was being evaluated for.",
      "rdfs:label": "cohort",
      "schema:domainIncludes": [
        {
          "@id": "cvisb:Patient"
        }
      ],
      "schema:rangeIncludes": [
        {
          "@id": "schema:Text"
        }
      ],
      "owl:cardinality": "one",
      "marginality": "required",
      "schema:Enumeration": [
        "Ebola",
        "Lassa",
        "COVID-19",
        "Control",
        "Unknown"
      ],
      "authenticated": false
    },
    {
      "@id": "cvisb:outcome",
      "@type": "rdf:Property",
      "rdfs:comment": "Outcome for patient: control, survivor, contact, dead, or unknown. Patients are considered survivors if they are alive at least 10 days after presentation of symptoms in the hospital, the time at which they are commonly discharged from the hospital.",
      "rdfs:label": "outcome",
      "schema:domainIncludes": [
        {
          "@id": "cvisb:Patient"
        }
      ],
      "schema:rangeIncludes": [
        {
          "@id": "schema:Text"
        }
      ],
      "owl:cardinality": "one",
      "marginality": "required",
      "schema:Enumeration": [
        "control",
        "survivor",
        "contact",
        "dead",
        "unknown"
      ],
      "authenticated": false
    },
    {
      "@id": "cvisb:country",
      "@type": "rdf:Property",
      "rdfs:comment": "Country where Patient was exposed to the virus",
      "rdfs:label": "country",
      "schema:domainIncludes": [
        {
          "@id": "cvisb:Patient"
        }
      ],
      "schema:rangeIncludes": [
        {
          "@id": "cvisb:Country"
        }
      ],
      "schema:sameAs": {
        "@id": "schema:geographicArea"
      },
      "owl:cardinality": "one",
      "marginality": "recommended",
      "authenticated": false
    },
    {
      "@id": "cvisb:location",
      "@type": "rdf:Property",
      "rdfs:comment": "The most specific geographic location of the patient. Could be a combination of country (Administrative Unit 0), district (Administrative Unit 2), chiefdom (Administrative Unit 3), Village/City name, and/or GPS coordinates. SHOULD ONLY INCLUDE LOCATIONS THAT CAN BE RELEASED TO THE PUBLIC.",
      "rdfs:label": "location",
      "schema:domainIncludes": [
        {
          "@id": "cvisb:Patient"
        }
      ],
      "schema:rangeIncludes": [
        {
          "@id": "cvisb:AdministrativeArea"
        }
      ],
      "schema:sameAs": {
        "@id": "schema:location"
      },
      "owl:cardinality": "many",
      "marginality": "recommended",
      "authenticated": false
    },
    {
      "@id": "cvisb:locationPrivate",
      "@type": "rdf:Property",
      "rdfs:comment": "The most specific geographic location of the patient. Could be a combination of country (Administrative Unit 0), district (Administrative Unit 2), chiefdom (Administrative Unit 3), Village/City name, and/or GPS coordinates.  Includes location information that should only be accessed by authorized users.",
      "rdfs:label": "locationPrivate",
      "schema:domainIncludes": [
        {
          "@id": "cvisb:Patient"
        }
      ],
      "schema:rangeIncludes": [
        {
          "@id": "cvisb:AdministrativeArea"
        }
      ],
      "schema:sameAs": {
        "@id": "schema:location"
      },
      "owl:cardinality": "many",
      "marginality": "recommended",
      "authenticated": true
    },
    {
      "@id": "cvisb:admittedLassaWard",
      "@type": "rdf:Property",
      "rdfs:comment": "Whether the patient was admitted to the Lassa isolation ward at KGH.",
      "rdfs:label": "admittedLassaWard",
      "schema:domainIncludes": [
        {
          "@id": "cvisb:Patient"
        }
      ],
      "schema:rangeIncludes": [
        {
          "@id": "schema:Boolean"
        }
      ],
      "owl:cardinality": "one",
      "marginality": "optional",
      "authenticated": true
    },
    {
      "@id": "cvisb:admitDate",
      "@type": "rdf:Property",
      "rdfs:comment": "Date of admission in the hospital. Note that not all patients who are evaluated are admitted for further care.",
      "rdfs:label": "admitDate",
      "schema:domainIncludes": [
        {
          "@id": "cvisb:Patient"
        }
      ],
      "schema:rangeIncludes": [
        {
          "@id": "schema:Date"
        }
      ],
      "owl:cardinality": "one",
      "marginality": "optional",
      "authenticated": true
    },
    {
      "@id": "cvisb:evalDate",
      "@type": "rdf:Property",
      "rdfs:comment": "Date of first evaluation in the hospital. Note that not all patients who are evaluated are admitted for further care.",
      "rdfs:label": "evalDate",
      "schema:domainIncludes": [
        {
          "@id": "cvisb:Patient"
        }
      ],
      "schema:rangeIncludes": [
        {
          "@id": "schema:Date"
        }
      ],
      "owl:cardinality": "one",
      "marginality": "optional",
      "authenticated": true
    },
    {
      "@id": "cvisb:presentationDate",
      "@type": "rdf:Property",
      "rdfs:comment": "Date of the first evaluation in the hospital; will be the minimum of the admitDate and evalDate",
      "rdfs:label": "presentationDate",
      "schema:domainIncludes": [
        {
          "@id": "cvisb:Patient"
        }
      ],
      "schema:rangeIncludes": [
        {
          "@id": "schema:Date"
        }
      ],
      "owl:cardinality": "one",
      "marginality": "optional",
      "authenticated": true
    },
    {
      "@id": "cvisb:presentationWeek",
      "@type": "rdf:Property",
      "rdfs:comment": "Week of presentation or first sample collection for the patient. Note that this date range could come from the date the patient was admitted to a health care facility, was evaluated, and/or a sample was collected and analyzed for them. This *may* be the week at which the patient was being treated in the acute phase of infection, or the date of first collection for a contact of an acutely ill patient, or it may be the date of a survivor follow-up visit where no data on their acute phase of illness is available.",
      "rdfs:label": "presentationWeek",
      "schema:domainIncludes": [
        {
          "@id": "cvisb:Patient"
        }
      ],
      "schema:rangeIncludes": [
        {
          "@id": "cvisb:DateRange"
        }
      ],
      "owl:cardinality": "one",
      "marginality": "recommended",
      "authenticated": false,
      "minimum": 1,
      "maximum": 52
    },
    {
      "@id": "cvisb:infectionYear",
      "@type": "rdf:Property",
      "rdfs:comment": "Approximate year of infection or contact with the virus. Based on self-reporting, so take it with a grain of salt.  If the onset of symptoms isn't reported, based on the date the patient presented in the hospital or was discharged.",
      "rdfs:label": "infectionYear",
      "schema:domainIncludes": [
        {
          "@id": "cvisb:Patient"
        }
      ],
      "schema:rangeIncludes": [
        {
          "@id": "schema:Integer"
        }
      ],
      "owl:cardinality": "one",
      "marginality": "optional",
      "authenticated": false
    },
    {
      "@id": "cvisb:infectionDate",
      "@type": "rdf:Property",
      "rdfs:comment": "Approximate date / date range of infection or contact with the virus. Based on self-reporting, so take it with a grain of salt.",
      "rdfs:label": "infectionDate",
      "schema:domainIncludes": [
        {
          "@id": "cvisb:Patient"
        }
      ],
      "schema:rangeIncludes": [
        {
          "@id": "schema:Date"
        }
      ],
      "owl:cardinality": "one",
      "marginality": "optional",
      "authenticated": true
    },
    {
      "@id": "cvisb:survivorEnrollmentDate",
      "@type": "rdf:Property",
      "rdfs:comment": "Date of enrollment of the survivor or contact in the KGH survivor study",
      "rdfs:label": "survivorEnrollmentDate",
      "schema:domainIncludes": [
        {
          "@id": "cvisb:Patient"
        }
      ],
      "schema:rangeIncludes": [
        {
          "@id": "schema:Date"
        }
      ],
      "owl:cardinality": "one",
      "marginality": "optional",
      "authenticated": true
    },
    {
      "@id": "cvisb:survivorEvalDates",
      "@type": "rdf:Property",
      "rdfs:comment": "Dates of evaluation of the survivor or contact in the KGH survivor study",
      "rdfs:label": "survivorEvalDates",
      "schema:domainIncludes": [
        {
          "@id": "cvisb:Patient"
        }
      ],
      "schema:rangeIncludes": [
        {
          "@id": "schema:Date"
        }
      ],
      "owl:cardinality": "many",
      "marginality": "optional",
      "authenticated": true
    },
    {
      "@id": "cvisb:dischargeDate",
      "@type": "rdf:Property",
      "rdfs:comment": "Date of discharge from the hospital",
      "rdfs:label": "dischargeDate",
      "schema:domainIncludes": [
        {
          "@id": "cvisb:Patient"
        }
      ],
      "schema:rangeIncludes": [
        {
          "@id": "schema:Date"
        }
      ],
      "owl:cardinality": "one",
      "marginality": "optional",
      "authenticated": true
    },
    {
      "@id": "cvisb:deathDate",
      "@type": "rdf:Property",
      "rdfs:comment": "Date of death",
      "rdfs:label": "deathDate",
      "schema:domainIncludes": [
        {
          "@id": "cvisb:Patient"
        }
      ],
      "schema:rangeIncludes": [
        {
          "@id": "schema:Date"
        }
      ],
      "owl:cardinality": "one",
      "marginality": "optional",
      "authenticated": true
    },
    {
      "@id": "cvisb:daysOnset",
      "@type": "rdf:Property",
      "rdfs:comment": "Number of days between onset of symptoms and hospital admission, as self-reported",
      "rdfs:label": "daysOnset",
      "schema:domainIncludes": [
        {
          "@id": "cvisb:Patient"
        }
      ],
      "schema:rangeIncludes": [
        {
          "@id": "schema:Integer"
        }
      ],
      "owl:cardinality": "one",
      "marginality": "optional",
      "authenticated": true
    },
    {
      "@id": "cvisb:daysInHospital",
      "@type": "rdf:Property",
      "rdfs:comment": "Number of days between first evaluation and discharge or death",
      "rdfs:label": "daysInHospital",
      "schema:domainIncludes": [
        {
          "@id": "cvisb:Patient"
        }
      ],
      "schema:rangeIncludes": [
        {
          "@id": "schema:Integer"
        }
      ],
      "owl:cardinality": "one",
      "marginality": "optional",
      "authenticated": true
    },
    {
      "@id": "cvisb:occupation",
      "@type": "rdf:Property",
      "rdfs:comment": "Occupation of patient",
      "rdfs:label": "occupation",
      "schema:domainIncludes": [
        {
          "@id": "cvisb:Patient"
        }
      ],
      "schema:rangeIncludes": [
        {
          "@id": "schema:Text"
        }
      ],
      "owl:cardinality": "one",
      "marginality": "optional",
      "authenticated": true
    },
    {
      "@id": "cvisb:gender",
      "@type": "rdf:Property",
      "rdfs:comment": "Gender",
      "rdfs:label": "gender",
      "schema:domainIncludes": [
        {
          "@id": "cvisb:Patient"
        }
      ],
      "schema:rangeIncludes": [
        {
          "@id": "schema:GenderType"
        }
      ],
      "schema:sameAs": {
        "@id": "schema:gender"
      },
      "owl:cardinality": "one",
      "marginality": "recommended",
      "schema:Enumeration": [
        "Male",
        "Female",
        "Unknown"
      ],
      "authenticated": false
    },
    {
      "@id": "cvisb:relatedTo",
      "@type": "rdf:Property",
      "rdfs:comment": "A list of related household contacts's public patientIDs",
      "rdfs:label": "relatedTo",
      "schema:domainIncludes": [
        {
          "@id": "cvisb:Patient"
        }
      ],
      "schema:rangeIncludes": [
        {
          "@id": "schema:Text"
        }
      ],
      "owl:cardinality": "many",
      "marginality": "optional",
      "authenticated": true
    },
    {
      "@id": "cvisb:relatedToPrivate",
      "@type": "rdf:Property",
      "rdfs:comment": "A list of related household contacts's private patientIDs",
      "rdfs:label": "relatedToPrivate",
      "schema:domainIncludes": [
        {
          "@id": "cvisb:Patient"
        }
      ],
      "schema:rangeIncludes": [
        {
          "@id": "schema:Text"
        }
      ],
      "owl:cardinality": "many",
      "marginality": "optional",
      "authenticated": true
    },
    {
      "@id": "cvisb:exposureType",
      "@type": "rdf:Property",
      "rdfs:comment": "For contacts, the type or level of exposure they had to the infected person.",
      "rdfs:label": "exposureType",
      "schema:domainIncludes": [
        {
          "@id": "cvisb:Patient"
        }
      ],
      "schema:rangeIncludes": [
        {
          "@id": "schema:Text"
        }
      ],
      "owl:cardinality": "one",
      "marginality": "optional",
      "authenticated": true
    },
    {
      "@id": "cvisb:contactSurvivorRelationship",
      "@type": "rdf:Property",
      "rdfs:comment": "For contacts, how they are related to the infected person.",
      "rdfs:label": "contactSurvivorRelationship",
      "schema:domainIncludes": [
        {
          "@id": "cvisb:Patient"
        }
      ],
      "schema:rangeIncludes": [
        {
          "@id": "schema:Text"
        }
      ],
      "owl:cardinality": "one",
      "marginality": "optional",
      "authenticated": true
    },
    {
      "@id": "cvisb:ethnicity",
      "@type": "rdf:Property",
      "rdfs:comment": "Patient ethnicity",
      "rdfs:label": "ethnicity",
      "schema:domainIncludes": [
        {
          "@id": "cvisb:Patient"
        }
      ],
      "schema:rangeIncludes": [
        {
          "@id": "schema:Text"
        }
      ],
      "owl:cardinality": "one",
      "marginality": "optional",
      "authenticated": true,
      "schema:Enumeration": [
        "Mende",
        "Fullah",
        "Temne",
        "Krio",
        "White",
        "Black",
        "Asian",
        "Other"
      ]
    },
    {
      "@id": "cvisb:age",
      "@type": "rdf:Property",
      "rdfs:comment": "Age at time of first presentation",
      "rdfs:label": "age",
      "schema:domainIncludes": [
        {
          "@id": "cvisb:Patient"
        }
      ],
      "schema:rangeIncludes": [
        {
          "@id": "schema:Float"
        },
        {
          "@id": "schema:Text"
        }
      ],
      "owl:cardinality": "one",
      "marginality": "recommended",
      "authenticated": false
    },
    {
      "@id": "cvisb:height",
      "@type": "rdf:Property",
      "rdfs:comment": "Patient height, in meters",
      "rdfs:label": "height",
      "schema:domainIncludes": [
        {
          "@id": "cvisb:Patient"
        }
      ],
      "schema:rangeIncludes": [
        {
          "@id": "schema:Float"
        }
      ],
      "owl:cardinality": "one",
      "marginality": "recommended",
      "authenticated": true
    },
    {
      "@id": "cvisb:weight",
      "@type": "rdf:Property",
      "rdfs:comment": "Patient weight, in kilograms",
      "rdfs:label": "weight",
      "schema:domainIncludes": [
        {
          "@id": "cvisb:Patient"
        }
      ],
      "schema:rangeIncludes": [
        {
          "@id": "schema:Float"
        }
      ],
      "owl:cardinality": "one",
      "marginality": "recommended",
      "authenticated": true
    },
    {
      "@id": "cvisb:pregnant",
      "@type": "rdf:Property",
      "rdfs:comment": "Whether the patient was pregnant at the time of presentation",
      "rdfs:label": "pregnant",
      "schema:domainIncludes": [
        {
          "@id": "cvisb:Patient"
        }
      ],
      "schema:rangeIncludes": [
        {
          "@id": "schema:Boolean"
        }
      ],
      "owl:cardinality": "one",
      "marginality": "recommended",
      "authenticated": true
    },
    {
      "@id": "cvisb:LassaExposed",
      "@type": "rdf:Property",
      "rdfs:comment": "Whether the patient was exposed to another person who had Lassa",
      "rdfs:label": "LassaExposed",
      "schema:domainIncludes": [
        {
          "@id": "cvisb:Patient"
        }
      ],
      "schema:rangeIncludes": [
        {
          "@id": "schema:Boolean"
        }
      ],
      "owl:cardinality": "one",
      "marginality": "recommended",
      "authenticated": true
    },
    {
      "@id": "cvisb:LassaHHDeaths",
      "@type": "rdf:Property",
      "rdfs:comment": "Whether the patient had recent Lassa-related deaths in their household",
      "rdfs:label": "LassaHHDeaths",
      "schema:domainIncludes": [
        {
          "@id": "cvisb:Patient"
        }
      ],
      "schema:rangeIncludes": [
        {
          "@id": "schema:Boolean"
        }
      ],
      "owl:cardinality": "one",
      "marginality": "recommended",
      "authenticated": true
    },
    {
      "@id": "cvisb:publisher",
      "@type": "rdf:Property",
      "rdfs:comment": "Publisher of the Patient demographic data",
      "rdfs:label": "publisher",
      "schema:domainIncludes": [
        {
          "@id": "cvisb:Patient"
        }
      ],
      "schema:rangeIncludes": [
        {
          "@id": "cvisb:Organization"
        }
      ],
      "schema:sameAs": {
        "@id": "schema:publisher"
      },
      "owl:cardinality": "one",
      "marginality": "recommended",
      "authenticated": false
    },
    {
      "@id": "cvisb:citation",
      "@type": "rdf:Property",
      "rdfs:comment": "Journal article or other publication associated with the patient demographic data (stored as an object, not a string).  If no citation exists (as in, the experiment hasn't been published yet), should be the publisher associated with the patient.",
      "rdfs:label": "citation",
      "schema:domainIncludes": [
        {
          "@id": "cvisb:Patient"
        }
      ],
      "schema:rangeIncludes": [
        {
          "@id": "cvisb:ScholarlyArticle"
        },
        {
          "@id": "cvisb:Organization"
        }
      ],
      "schema:sameAs": {
        "@id": "schema:citation"
      },
      "owl:cardinality": "many",
      "marginality": "recommended",
      "authenticated": false
    },
    {
      "@id": "cvisb:correction",
      "@type": "rdf:Property",
      "rdfs:comment": "A list of the changes made to the Patient metadata. Optional, but useful to tag when and/or why specific fields were changed.",
      "rdfs:label": "correction",
      "schema:domainIncludes": [
        {
          "@id": "cvisb:Patient"
        }
      ],
      "schema:rangeIncludes": [
        {
          "@id": "schema:Text"
        }
      ],
      "schema:sameAs": {
        "@id": "schema:correction"
      },
      "owl:cardinality": "many",
      "marginality": "recommended",
      "authenticated": false
    },
    {
      "@id": "cvisb:symptoms",
      "@type": "rdf:Property",
      "rdfs:comment": "List of symptoms the patient experienced during or after the course of illness.",
      "rdfs:label": "symptoms",
      "schema:domainIncludes": [
        {
          "@id": "cvisb:Patient"
        }
      ],
      "schema:rangeIncludes": [
        {
          "@id": "cvisb:Symptom"
        }
      ],
      "owl:cardinality": "many",
      "marginality": "recommended",
      "authenticated": false
    },
    {
      "@id": "cvisb:medications",
      "@type": "rdf:Property",
      "rdfs:comment": "List of medications administered (or not) to the patient during the course of their treatment.",
      "rdfs:label": "medications",
      "schema:domainIncludes": [
        {
          "@id": "cvisb:Patient"
        }
      ],
      "schema:rangeIncludes": [
        {
          "@id": "cvisb:Medication"
        }
      ],
      "owl:cardinality": "many",
      "marginality": "recommended",
      "authenticated": false
    },
    {
      "@id": "cvisb:elisa",
      "@type": "rdf:Property",
      "rdfs:comment": "List of ELISA results (IgG, IgM, Ag for Ebola/Lassa antigen) for the patient",
      "rdfs:label": "elisa",
      "schema:domainIncludes": [
        {
          "@id": "cvisb:Patient"
        }
      ],
      "schema:rangeIncludes": [
        {
          "@id": "cvisb:ELISA"
        }
      ],
      "owl:cardinality": "many",
      "marginality": "recommended",
      "authenticated": false
    },
    {
      "@id": "cvisb:Organization",
      "@type": "rdfs:Class",
      "rdfs:comment": "A schema describing an Organization for the Center for Viral Systems Biology",
      "rdfs:label": "Organization",
      "rdfs:subClassOf": {
        "@id": "schema:Organization"
      },
      "schema:isPartOf": {
        "@id": "https://data.cvisb.org/schema"
      },
      "schema:sameAs": {
        "@id": "schema:Organization"
      }
    },
    {
      "@id": "cvisb:name",
      "@type": "rdf:Property",
      "rdfs:comment": "Descriptive name of the Organization",
      "rdfs:label": "name",
      "schema:domainIncludes": [
        {
          "@id": "cvisb:Organization"
        }
      ],
      "schema:rangeIncludes": [
        {
          "@id": "xsd:string"
        },
        {
          "@id": "schema:Text"
        }
      ],
      "schema:sameAs": {
        "@id": "schema:name"
      },
      "owl:cardinality": "one",
      "marginality": "required",
      "authenticated": false
    },
    {
      "@id": "cvisb:identifier",
      "@type": "rdf:Property",
      "rdfs:comment": "Unique identifier of the Organization",
      "rdfs:label": "identifier",
      "schema:domainIncludes": [
        {
          "@id": "cvisb:Organization"
        }
      ],
      "schema:rangeIncludes": [
        {
          "@id": "xsd:string"
        },
        {
          "@id": "schema:Text"
        }
      ],
      "schema:sameAs": {
        "@id": "schema:identifier"
      },
      "owl:cardinality": "one",
      "marginality": "recommended",
      "authenticated": false
    },
    {
      "@id": "cvisb:alternateName",
      "@type": "rdf:Property",
      "rdfs:comment": "Alternate name of the Organization",
      "rdfs:label": "alternateName",
      "schema:domainIncludes": [
        {
          "@id": "cvisb:Organization"
        }
      ],
      "schema:rangeIncludes": [
        {
          "@id": "xsd:string"
        },
        {
          "@id": "schema:Text"
        }
      ],
      "schema:sameAs": {
        "@id": "schema:alternateName"
      },
      "owl:cardinality": "many",
      "marginality": "optional",
      "authenticated": false
    },
    {
      "@id": "cvisb:description",
      "@type": "rdf:Property",
      "rdfs:comment": "Description of the Organization",
      "rdfs:label": "description",
      "schema:domainIncludes": [
        {
          "@id": "cvisb:Organization"
        }
      ],
      "schema:rangeIncludes": [
        {
          "@id": "xsd:string"
        },
        {
          "@id": "schema:Text"
        }
      ],
      "schema:sameAs": {
        "@id": "schema:description"
      },
      "owl:cardinality": "one",
      "marginality": "recommended",
      "authenticated": false
    },
    {
      "@id": "cvisb:url",
      "@type": "rdf:Property",
      "rdfs:comment": "URL of the Organization",
      "rdfs:label": "url",
      "schema:domainIncludes": [
        {
          "@id": "cvisb:Organization"
        }
      ],
      "schema:rangeIncludes": [
        {
          "@id": "xsd:string"
        },
        {
          "@id": "schema:Text"
        }
      ],
      "schema:sameAs": {
        "@id": "schema:url"
      },
      "owl:cardinality": "one",
      "marginality": "recommended",
      "authenticated": false
    },
    {
      "@id": "cvisb:email",
      "@type": "rdf:Property",
      "rdfs:comment": "email of the Organization; could also be specified in contactPoint",
      "rdfs:label": "email",
      "schema:domainIncludes": [
        {
          "@id": "cvisb:Organization"
        }
      ],
      "schema:rangeIncludes": [
        {
          "@id": "xsd:string"
        },
        {
          "@id": "schema:Text"
        }
      ],
      "schema:sameAs": {
        "@id": "schema:email"
      },
      "owl:cardinality": "one",
      "marginality": "optional"
    },
    {
      "@id": "cvisb:parentOrganization",
      "@type": "rdf:Property",
      "rdfs:comment": "The larger organization that this organization is a subOrganization of, if any",
      "rdfs:label": "parentOrganization",
      "schema:domainIncludes": [
        {
          "@id": "cvisb:Organization"
        }
      ],
      "schema:rangeIncludes": [
        {
          "@id": "schema:Text"
        }
      ],
      "schema:sameAs": {
        "@id": "schema:parentOrganization"
      },
      "owl:cardinality": "one",
      "marginality": "optional",
      "authenticated": false
    },
    {
      "@id": "cvisb:logo",
      "@type": "rdf:Property",
      "rdfs:comment": "logo for the organization",
      "rdfs:label": "logo",
      "schema:domainIncludes": [
        {
          "@id": "cvisb:Organization"
        }
      ],
      "schema:rangeIncludes": [
        {
          "@id": "schema:URL"
        }
      ],
      "schema:sameAs": {
        "@id": "schema:logo"
      },
      "owl:cardinality": "one",
      "marginality": "optional",
      "authenticated": false
    },
    {
      "@id": "cvisb:contactPoint",
      "@type": "rdf:Property",
      "rdfs:comment": "Contact point for the Organization",
      "rdfs:label": "contactPoint",
      "schema:domainIncludes": [
        {
          "@id": "cvisb:Organization"
        }
      ],
      "schema:rangeIncludes": [
        {
          "@id": "cvisb:ContactPoint"
        }
      ],
      "schema:sameAs": {
        "@id": "schema:contactPoint"
      },
      "owl:cardinality": "one",
      "marginality": "recommended",
      "authenticated": false
    },
    {
      "@id": "cvisb:address",
      "@type": "rdf:Property",
      "rdfs:comment": "Postal address for the Organization",
      "rdfs:label": "address",
      "schema:domainIncludes": [
        {
          "@id": "cvisb:Organization"
        }
      ],
      "schema:rangeIncludes": [
        {
          "@id": "cvisb:PostalAddress"
        }
      ],
      "schema:sameAs": {
        "@id": "schema:address"
      },
      "owl:cardinality": "one",
      "marginality": "optional",
      "authenticated": false
    },
    {
      "@id": "cvisb:@type",
      "@type": "rdf:Property",
      "rdfs:comment": "Type, used for internal purposes; should be Organization",
      "rdfs:label": "@type",
      "schema:domainIncludes": [
        {
          "@id": "cvisb:Organization"
        }
      ],
      "schema:rangeIncludes": [
        {
          "@id": "schema:Text"
        }
      ],
      "owl:cardinality": "one",
      "marginality": "recommended",
      "authenticated": false,
      "schema:Enumeration": [
        "Organization"
      ]
    },
    {
      "@id": "cvisb:OxygenSaturation",
      "@type": "rdfs:Class",
      "rdfs:comment": "A schema describing a single oxygen saturation datapoint collected from patients in the Center for Viral Systems Biology.",
      "rdfs:label": "OxygenSaturation",
      "rdfs:subClassOf": {
        "@id": "cvisb:Data"
      },
      "schema:isPartOf": {
        "@id": "https://data.cvisb.org/schema"
      }
    },
    {
      "@id": "cvisb:@type",
      "@type": "rdf:Property",
      "rdfs:comment": "Type of data",
      "rdfs:label": "@type",
      "schema:domainIncludes": [
        {
          "@id": "cvisb:OxygenSaturation"
        }
      ],
      "schema:rangeIncludes": [
        {
          "@id": "schema:Text"
        }
      ],
      "owl:cardinality": "one",
      "marginality": "required",
      "authenticated": false,
      "schema:Enumeration": [
        "OxygenSaturation"
      ]
    },
    {
      "@id": "cvisb:time",
      "@type": "rdf:Property",
      "rdfs:comment": "Date and time of OxygenSaturation measurement",
      "rdfs:label": "time",
      "schema:domainIncludes": [
        {
          "@id": "cvisb:OxygenSaturation"
        }
      ],
      "schema:rangeIncludes": [
        {
          "@id": "schema:DateTime"
        }
      ],
      "owl:cardinality": "one",
      "marginality": "recommended",
      "authenticated": true
    },
    {
      "@id": "cvisb:oxygenSaturation",
      "@type": "rdf:Property",
      "rdfs:comment": "OxygenSaturation, in percent",
      "rdfs:label": "oxygenSaturation",
      "schema:domainIncludes": [
        {
          "@id": "cvisb:OxygenSaturation"
        }
      ],
      "schema:rangeIncludes": [
        {
          "@id": "schema:Float"
        }
      ],
      "owl:cardinality": "one",
      "marginality": "required",
      "authenticated": true
    },
    {
      "@id": "cvisb:collectionInstrument",
      "@type": "rdf:Property",
      "rdfs:comment": "Whether the measurement was recorded using a PhysIQ sensor or a conventional measurement by a nurse/doctor",
      "rdfs:label": "collectionInstrument",
      "schema:domainIncludes": [
        {
          "@id": "cvisb:OxygenSaturation"
        }
      ],
      "schema:rangeIncludes": [
        {
          "@id": "schema:Text"
        }
      ],
      "owl:cardinality": "one",
      "marginality": "recommended",
      "authenticated": true,
      "schema:Enumeration": [
        "PhysIQ",
        "conventional"
      ]
    },
    {
      "@id": "cvisb:Person",
      "@type": "rdfs:Class",
      "rdfs:comment": "A schema describing a Person in the Center for Viral Systems Biology, mostly for the purposes of authorship of papers",
      "rdfs:label": "Person",
      "rdfs:subClassOf": {
        "@id": "schema:Person"
      },
      "schema:isPartOf": {
        "@id": "https://data.cvisb.org/schema"
      },
      "schema:sameAs": {
        "@id": "schema:Person"
      }
    },
    {
      "@id": "cvisb:givenName",
      "@type": "rdf:Property",
      "rdfs:comment": "Given name. In the U.S., the first name of a Person. This can be used along with familyName instead of the name property.",
      "rdfs:label": "givenName",
      "schema:domainIncludes": [
        {
          "@id": "cvisb:Person"
        }
      ],
      "schema:rangeIncludes": [
        {
          "@id": "schema:Text"
        }
      ],
      "schema:sameAs": {
        "@id": "schema:Person"
      },
      "owl:cardinality": "one",
      "marginality": "recommended",
      "authenticated": false
    },
    {
      "@id": "cvisb:additionalName",
      "@type": "rdf:Property",
      "rdfs:comment": "An additional name for a Person, can be used for a middle name",
      "rdfs:label": "additionalName",
      "schema:domainIncludes": [
        {
          "@id": "cvisb:Person"
        }
      ],
      "schema:rangeIncludes": [
        {
          "@id": "schema:Text"
        }
      ],
      "schema:sameAs": {
        "@id": "schema:Person"
      },
      "owl:cardinality": "one",
      "marginality": "recommended",
      "authenticated": false
    },
    {
      "@id": "cvisb:familyName",
      "@type": "rdf:Property",
      "rdfs:comment": "Family name. In the U.S., the last name of an Person. This can be used along with givenName instead of the name property.",
      "rdfs:label": "familyName",
      "schema:domainIncludes": [
        {
          "@id": "cvisb:Person"
        }
      ],
      "schema:rangeIncludes": [
        {
          "@id": "schema:Text"
        }
      ],
      "schema:sameAs": {
        "@id": "schema:Person"
      },
      "owl:cardinality": "one",
      "marginality": "recommended",
      "authenticated": false
    },
    {
      "@id": "cvisb:name",
      "@type": "rdf:Property",
      "rdfs:comment": "Full name of the person-- concatenation of givenName, additionalName, familyName. givenName, additionalName, and familyName are the preferred way of specifying the name.",
      "rdfs:label": "name",
      "schema:domainIncludes": [
        {
          "@id": "cvisb:Person"
        }
      ],
      "schema:rangeIncludes": [
        {
          "@id": "schema:Text"
        }
      ],
      "schema:sameAs": {
        "@id": "schema:Person"
      },
      "owl:cardinality": "one",
      "marginality": "recommended",
      "authenticated": false
    },
    {
      "@id": "cvisb:MonetaryGrant",
      "@type": "rdfs:Class",
      "rdfs:comment": "A schema describing the MonetaryGrant for the Center for Viral Systems Biology",
      "rdfs:label": "MonetaryGrant",
      "rdfs:subClassOf": {
        "@id": "schema:MonetaryGrant"
      },
      "schema:isPartOf": {
        "@id": "https://data.cvisb.org/schema"
      },
      "schema:sameAs": {
        "@id": "schema:MonetaryGrant"
      }
    },
    {
      "@id": "cvisb:funder",
      "@type": "rdf:Property",
      "rdfs:comment": "Descriptive name of the MonetaryGrant",
      "rdfs:label": "funder",
      "schema:domainIncludes": [
        {
          "@id": "cvisb:MonetaryGrant"
        }
      ],
      "schema:rangeIncludes": [
        {
          "@id": "cvisb:Organization"
        }
      ],
      "schema:sameAs": {
        "@id": "schema:funder"
      },
      "owl:cardinality": "one",
      "marginality": "required",
      "authenticated": false
    },
    {
      "@id": "cvisb:identifier",
      "@type": "rdf:Property",
      "rdfs:comment": "Unique identifier for the grant, e.g. U19AI135995 for CViSB's NIAID U19 award.",
      "rdfs:label": "identifier",
      "schema:domainIncludes": [
        {
          "@id": "cvisb:MonetaryGrant"
        }
      ],
      "schema:rangeIncludes": [
        {
          "@id": "schema:Text"
        }
      ],
      "schema:sameAs": {
        "@id": "schema:identifier"
      },
      "owl:cardinality": "one",
      "marginality": "required",
      "authenticated": false
    }
  ]
}